theories/Ordered6/Monad.v
@@ -1,0 +1,50 @@
+Require Export PredMonad.Ordered6.OrderedType.
+
+Import OTNotations.
+
+
+(***
+ *** The monad typeclass
+ ***)
+
+Class MonadOps (M: OType -> OType) : Type :=
+  { returnM : forall {A}, A -o> M A;
+    bindM : forall {A B}, M A -o> (A -o> M B) -o> M B }.
+
+Class Monad M `{MOps:MonadOps M} : Prop :=
+  {
+    monad_return_bind :
+      forall A B (f: A -o> M B) x,
+        bindM @o@ (returnM @o@ x) @o@ f =o= f @o@ x;
+
+    monad_bind_return :
+      forall A (m : M A), bindM @o@ m @o@ returnM =o= m;
+
+    monad_assoc :
+      forall A B C m (f: A -o> M B) (g: B -o> M C),
+        bindM @o@ (bindM @o@ m @o@ f) @o@ g
+        =o=
+        bindM @o@ m @o@ (mkOTerm _ (fun x => bindM @o@ (f @o@ x) @o@ g));
+  }.
+
+(* Helpful bind notation *)
+Notation "'do' x <- m1 ; m2" :=
+  (bindM @o@ m1 @o@ (mkOTerm _ (fun x => m2))) (at level 60, right associativity).
+
+
+(***
+ *** The Identity Monad
+ ***)
+
+Definition Identity (A:OType) := A.
+
+Instance IdMonad_MonadOps : MonadOps Identity :=
+  { returnM := fun A => mkOTerm (A -o> Identity A) (fun x => x);
+    bindM := fun A B =>
+               mkOTerm (A -o> (A -o> B) -o> B)
+                       (fun m (f:Pfun A B) => f @o@ m) }.
+
+Instance IdMonad : Monad Identity.
+Proof.
+  constructor; intros; simpl; reflexivity.
+Qed.
