theories/Ordered6/MonadState.v
@@ -1,0 +1,103 @@
+Require Export PredMonad.Ordered6.Monad.
+
+Import OTNotations.
+
+
+(***
+ *** Monads with State Effects
+ ***)
+
+(* State effects = get and put *)
+Class MonadStateOps M `{MOps:MonadOps M} (St:OType) : Type :=
+  {
+    getM : M St ;
+    putM : St -o> M OTunit
+  }.
+
+Class MonadState M `{MSOps:MonadStateOps M} : Prop :=
+  {
+    monad_state_monad :> Monad M;
+
+    monad_state_get :
+      forall A (m : M A),
+        bindM @o@ getM @o@ (mkOTerm _ (fun _ => m)) =o= m ;
+
+    monad_state_get_put :
+      forall A (f : St -o> OTunit -o> M A),
+        bindM @o@ getM @o@
+              (mkOTerm (St -o> M A)
+                       (fun s => bindM @o@ (putM @o@ s) @o@ (f @o@ s)))
+        =o= bindM @o@ getM @o@
+                  (mkOTerm (St -o> M A) (fun s => f @o@ s @o@ tt)) ;
+
+    monad_state_put_get :
+      forall A s (f : OTunit -o> St -o> M A),
+        bindM @o@ (putM @o@ s) @o@
+              (mkOTerm (OTunit -o> M A) (fun u => bindM @o@ getM @o@ (f @o@ u)))
+        =o= bindM @o@ (putM @o@ s) @o@
+                  (mkOTerm (OTunit -o> M A) (fun u => f @o@ u @o@ s)) ;
+
+    monad_state_put_put :
+      forall A s1 s2 (f : OTunit -o> OTunit -o> M A),
+        bindM @o@ (putM @o@ s1) @o@
+              (mkOTerm (OTunit -o> M A)
+                       (fun u => bindM @o@ (putM @o@ s2) @o@ (f @o@ u)))
+        =o= bindM @o@ (putM @o@ s2) @o@ (f @o@ tt)
+  }.
+
+
+(***
+ *** The State Monad Transformer
+ ***)
+
+Definition StateT St M A := St -o> M (St *o* A).
+
+Set Printing All. Typeclasses eauto := debug.
+Instance StateT_MonadOps St M (MOps:MonadOps M) : MonadOps (StateT St M) :=
+  {returnM :=
+     fun A => mkOTerm (A -o> St -o> M (St *o* A))
+                      (fun x s => returnM @o@ (s ,o, x));
+
+   bindM :=
+     fun A B =>
+       mkOTerm _ (fun (m:StateT St M A) (f:A -o> StateT St M B) s =>
+                    do s_x <- (m @o@ s);
+                      f @o@ (osnd @o@ s_x) @o@ (ofst @o@ s_x))
+  }.
+
+(* The Monad instance for StateT *)
+Global Instance StateT_Monad : Monad (StateT).
+Proof.
+  constructor; intros; unfold StateT, returnM, bindM, lrM, StateT_MonadOps.
+  - auto with typeclass_instances.
+  - prove_lr_proper.
+  - prove_lr_proper.
+  - intros R1 R2 subR; apply LRFun_Proper_subrelation; apply monad_proper_lrM;
+      apply LRPair_Proper_subrelation; try assumption; reflexivity.
+  - prove_lr.
+  - transitivity (fun s => do s_x <- m s; returnM s_x).
+    + split; build_lr_fun; apply monad_proper_bind; prove_lr.
+    + prove_lr; autorewrite with LR; prove_lr.
+  - prove_lr.
+Qed.
+
+Global Instance StateT_MonadStateOps : MonadStateOps S StateT :=
+  { getM := fun s => returnM (s, s)
+  ; putM := fun s _ => returnM (s, tt)
+  }.
+
+Global Instance StateT_MonadState : MonadState S StateT.
+Proof.
+  constructor; intros;
+    unfold StateT, returnM, bindM, lrM, getM, putM,
+    StateT_MonadOps, StateT_MonadStateOps.
+  - auto with typeclass_instances.
+  - prove_lr_proper.
+  - prove_lr_proper.
+  - prove_lr.
+  - prove_lr.
+  - prove_lr.
+  - prove_lr.
+Qed.
+
+End StateT.
